src/FJ/ClassTable.v
@@ -2,7 +2,7 @@ Require Import Decidable Relations.
 Require Import Base.
 Require Import FJ.Syntax.
 
-(* We assume a fixed CT *)
+(* We assume a fixed Class Table*)
 Parameter CT: [Class].
 
 Reserved Notation "C '<:' D " (at level 40).
@@ -23,27 +23,6 @@ Tactic Notation "subtype_cases" tactic(first) ident(c) :=
   [ Case_aux c "S_Refl" | Case_aux c "S_Trans" 
   | Case_aux c "S_Decl"].
 
-Fixpoint succ (C: Class) ct : option ClassRefinement :=
-  match ct with
-  | nil => None
-  | c :: cs => 
-   match c with 
-    | CD _ => succ C cs
-    | CR CRef => 
-     match CRef with
-      | CRefine C' _ 0 _ _ _ _ _ => if beq_id (ref C) C' then Some CRef else None
-      | CRefine _ _ (S n) _ _ _ _ _ => succ C cs
-    end
-  end
-  end.
-
-Fixpoint succ : ClassName -> ClassName :=
-  match CT with
-  | nil => Object
-  | c :: cs => match c with 
-               | CD (CDecl id _ _ _ _ _ _) =>
-               | CR (CRefine id _ _ _ _ _ _ _) => 
-
 (* Hypothesis for ClassTable sanity *)
 Module CTSanity.
 Hypothesis dec_subtype: forall C D,
@@ -52,17 +31,12 @@ Hypothesis dec_subtype: forall C D,
 Hypothesis antisym_subtype:
   antisymmetric _ Subtype.
 
-Hypothesis ClassesOK: forall C D Fs noDupfs K Ms noDupMds, 
-  find C CT = Some (CDecl C D Fs noDupfs K Ms noDupMds) ->
-  CType_OK (CDecl C D Fs noDupfs K Ms noDupMds).
-Hint Resolve ClassesOK.
-
 Hypothesis obj_notin_dom: find Object CT = None.
 Hint Rewrite obj_notin_dom.
 
 Hypothesis superClass_in_dom: forall C D Fs noDupfs K Ms noDupMds,
-  find C CT = Some (CDecl C D Fs noDupfs K Ms noDupMds) ->
+  find C CT = Some (CD (CDecl C D Fs noDupfs K Ms noDupMds)) ->
   D <> Object ->
-  exists D0 Fs0 noDupfs0 K0 Ms0 noDupMds0, find D CT = Some (CDecl D D0 Fs0 noDupfs0 K0 Ms0 noDupMds0).
+  exists D0 Fs0 noDupfs0 K0 Ms0 noDupMds0, find D CT = Some (CD (CDecl D D0 Fs0 noDupfs0 K0 Ms0 noDupMds0)).
 
 End CTSanity.
