src/FJ/RefinementTable.v
@@ -1,0 +1,40 @@
+Require Import Decidable Relations.
+Require Import Base.
+Require Import FJ.Syntax.
+Require Import FJ.ClassTable.
+
+(* A fixed Refinement Table*)
+Parameter RT: ClassRefinement -> RefinementName.
+
+Definition isRefinement (C: Class): bool:=
+  match C with
+  | CD _ => false
+  | CR _ => true
+  end.
+
+Definition RefT := filter isRefinement CT.
+
+
+Inductive succ: Class -> ClassRefinement -> Prop :=
+  | S_Decl : forall (C: Class) (C': CRefinement),
+    C' = (CRefine _ ft' _ _ _ _ _) ->
+    
+
+Fixpoint suc (C: ClassName) ft ct : option ClassRefinement :=
+  match ct with
+  | nil => None
+  | c :: cs => 
+   match c with 
+    | CD _ => suc C ft cs
+    | CR ((CRefine C' ft' _ _ _ _ _) as CRef) => 
+     match beq_id C C' with
+      | true => if lt_dec ft ft' then Some CRef else suc C ft cs
+      | false => suc C ft cs
+     end
+   end
+  end.
+
+Definition succ (C: Class) : option ClassRefinement :=
+  match C with
+  | CD CDec => suc (ref CDec) 0 CT
+  | CR (CRefi
